Tests/type_inference/local_constraints.ml
@@ -1,0 +1,9 @@
+open Mica
+
+let _ =
+  let inferred_list : int list =
+    let xs = [] in
+    4 :: xs
+  in
+  let _ = List.length inferred_list in
+  ()
