Tests/type_inference/specified_incomplete.ml
@@ -1,0 +1,5 @@
+(* TEST: no-compile *)
+open Mica
+
+let bad x : int = x
+[@@spec fun x -> ret (fun r -> assert (r = x))]
