Tests/type_inference/unequal_application.ml
@@ -1,0 +1,4 @@
+(* TEST: no-compile *)
+open Mica
+
+let bad = List.length true
