Tests/type_inference/unequal_constructor.ml
@@ -1,0 +1,4 @@
+(* TEST: no-compile *)
+open Mica
+
+let bad : int option = Some true
