Mica/Base/Except.lean
@@ -23,4 +23,13 @@ theorem bind_ok {σ ε α β} {f : StateT σ (Except ε) α} {g : α → StateT 
   have ⟨p, hf, hg⟩ := Except.bind_ok h
   exact ⟨p.1, p.2, hf, hg⟩
 
+theorem bind_ok₂ {σ₁ σ₂ ε α β}
+    {f : StateT σ₁ (StateT σ₂ (Except ε)) α} {g : α → StateT σ₁ (StateT σ₂ (Except ε)) β}
+    {s₁ s₁' : σ₁} {s₂ s₂' : σ₂} {b : β}
+    (h : (f >>= g) s₁ s₂ = .ok ((b, s₁'), s₂')) :
+    ∃ a t₁ t₂, f s₁ s₂ = .ok ((a, t₁), t₂) ∧ g a t₁ t₂ = .ok ((b, s₁'), s₂') := by
+  have h' : (f s₁ >>= fun p => g p.1 p.2) s₂ = .ok ((b, s₁'), s₂') := h
+  have ⟨p, s₀, hf, hg⟩ := StateT.bind_ok h'
+  exact ⟨p.1, p.2, s₀, hf, hg⟩
+
 end StateT
